theories/encryption/Indist.ec
@@ -19,6 +19,10 @@ clone import Hybrid as H
   with type input <- input * input,
        type outputA <- bool.
 
+(* Specialize Hybrid argument to oracle that takes
+   two arguments and either uses first argument (left)
+   or second argument (right). *)
+
 module type Orcl = {
   proc leaks (il:inleaks) : outleaks  
   proc orcl (m:input) : output
@@ -32,8 +36,8 @@ module OrclL (O:Orcl) = {
 
   proc orcl (m0 m1:input) : output = {
     var r : output;
-    r = O.orcl(m0);
-    C.incr();
+    r <@ O.orcl(m0);
+    Count.incr();
     return r;
   }
 }.
@@ -41,31 +45,22 @@ module OrclL (O:Orcl) = {
 module OrclR (O:Orcl) = {
   proc orcl (m0 m1:input) : output = {
     var r : output;
-    C.incr();
-    r = O.orcl(m1);
+    Count.incr();
+    r <@ O.orcl(m1);
     return r;
   }
 }.
 
-module Orclb (O:Orcl) = {
-
-  var b:bool
-  proc orcl (m0 m1:input) : output = {
-    var r : output;
-    C.incr();
-    r = O.orcl(b?m0:m1);
-    return r;
-  }
+module type Adv (O:Orcl, LR:LR) = {
+  proc main():bool { O.leaks O.orcl LR.orcl }
 }.
-
-module type Adv (O:Orcl, LR:LR) = { proc main():bool { O.leaks O.orcl LR.orcl }}.
 
 module INDL (O:Orcl, A:Adv) = {
   module A = A(O,OrclL(O))
   proc main():bool = {
     var b' : bool;
-    C.init();
-    b' = A.main();
+    Count.init();
+    b' <@ A.main();
     return b';
   }
 }.
@@ -74,123 +69,48 @@ module INDR (O:Orcl, A:Adv) = {
   module A = A(O,OrclR(O))
   proc main():bool = {
     var b' : bool;
-    C.init();
-    b' = A.main();
+    Count.init();
+    b' <@ A.main();
     return b';
   }
 }.
 
-module INDb(O:Orcl,A:Adv) = {
-  module A = A(O,Orclb(O))
-  proc main():bool = {
-    var b' : bool;
-    C.init();
-    Orclb.b = ${0,1};
-    b' = A.main();
-    return Orclb.b = b';
-  }
-}.
-
-(* We prove the equivalence between the two usual definitions *)
-(* i.e (INDb - 1/2) = (INDL - INDR)/2 *)
-
-section.
-  declare module O:Orcl {C, Orclb}.
-  declare module A:Adv  {C, O, Orclb}.
-
-  local module WA = {
-    module A=A(O,Orclb(O))  
-    proc work(x:bool) : bool = {
-      var b' : bool;
-      C.init();
-      Orclb.b = x;
-      b' = A.main();
-      return b';
-    }
-  }.
-
-  lemma INDb_INDLR &m (p:glob A -> glob O -> int -> bool):
-     Pr[INDb(O,A).main() @ &m : res /\ p (glob A) (glob O) C.c] -
-       Pr[INDR(O,A).main() @ &m : p (glob A) (glob O) C.c]/2%r =
-     (Pr[INDL(O,A).main() @ &m : res /\ p (glob A) (glob O) C.c] -
-      Pr[INDR(O,A).main() @ &m : res /\ p (glob A) (glob O) C.c])/2%r.
-  proof strict.
-   cut := Sample_bool WA &m 
-     (fun (g:glob WA), let (b,c,ga,go) = g in p ga go c) => /= H.
-   cut -> : Pr[INDb(O, A).main() @ &m : res /\ p (glob A) (glob O) C.c] =
-    Pr[MB.M.Rand(WA).main() @ &m : fst res = snd res /\ p (glob A) (glob O) C.c].
-     byequiv (_: ={glob A,glob O} ==> ={glob A,glob O, C.c} /\
-                   res{1} = (fst res = snd res){2}) => //;proc.
-     inline C.init WA.work;simplify fst snd. 
-     by swap{1} 2 -1; sim; proc (={Orclb.b, C.c}).
-   cut He: equiv [INDR(O, A).main ~ WA.work: x{2}=false /\ 
-                   ={glob A,glob O} ==> ={res,glob A,glob O, C.c}].
-    proc. 
-    call (_: ={glob O, C.c} /\ Orclb.b{2} = false).
-      by proc (={C.c} /\ Orclb.b{2} = false).      
-      by proc (={C.c} /\ Orclb.b{2} = false). 
-      by proc;inline C.incr;wp;call(_:true);wp;skip;progress.
-    inline C.init;by wp.
-   cut -> : Pr[INDR(O, A).main() @ &m : p (glob A) (glob O) C.c] =
-            Pr[WA.work(false) @ &m : p (glob A) (glob O) C.c].
-     by byequiv He.
-   cut -> : Pr[INDR(O, A).main() @ &m : res /\ p (glob A) (glob O) C.c] = 
-            Pr[WA.work(false) @ &m : res /\ p (glob A) (glob O) C.c].
-     by byequiv He.
-   (cut -> : Pr[INDL(O, A).main() @ &m : res /\ p (glob A) (glob O) C.c] = 
-            Pr[WA.work(true) @ &m : res /\ p (glob A) (glob O) C.c]) => //.
-   byequiv 
-      (_: x{2}=true /\ ={glob A,glob O} ==> ={res,glob A,glob O, C.c}) => //.
-   proc; call (_: ={glob O, C.c} /\ Orclb.b{2} = true).
-     by proc (={C.c} /\ Orclb.b{2} = true).      
-     by proc (={C.c} /\ Orclb.b{2} = true). 
-     by proc;inline C.incr;wp;call(_:true);wp;skip;progress.
-   inline C.init;by wp.
- qed.
-
-end section.
-
+(* -------------------------------------------------------------------- *)
 (* We prove that IND-n is equivalent to IND-1 *)
 
 module Orcl2(O:Orcl) = {
-  proc leaks (il:inleaks) : outleaks = {
-    var r : outleaks;
-    r = O.leaks(il);
-    return r;
-  }
+  proc leaks = O.leaks
 
-  proc orcl1 (m:input * input) : output = {
-    var r : output;
+  proc orclL(m : input * input) : output = {
+    var r;
     r = O.orcl(fst m);
     return r;
   }
 
-  proc orcl2 (m:input * input) : output = {
-    var r : output;
+  proc orclR(m : input * input) : output = {
+    var r;
     r = O.orcl(snd m);
     return r;
-  }  
+  }
 }.
 
-module LRB2 (O:Orcl,LR:LR) = {
+module HybOrcl2 (O:Orcl,LR:LR) = {
   proc orcl(m0 m1:input):output = {
     var r : output;
-    if (LRB.l0 < LRB.l) r = O.orcl(m0);
-    else { 
-      if (LRB.l0 = LRB.l) r = LR.orcl(m0,m1);
-      else r = O.orcl(m1);
-    }
-    LRB.l = LRB.l + 1;
+    if   (HybOrcl.l0 < HybOrcl.l) r <@ O.orcl(m0);
+    elif (HybOrcl.l0 = HybOrcl.l) r <@ LR.orcl(m0,m1);
+    else                          r <@ O.orcl(m1);
+    HybOrcl.l = HybOrcl.l + 1;
     return r;
-  }    
+  }
 }.
 
-module B(A:Adv, O:Orcl, LR:LR) = {
-  module A = A(O,LRB2(O,LR))
+module HybGame2(A:Adv, O:Orcl, LR:LR) = {
+  module A = A(O,HybOrcl2(O,LR))
   proc main():bool = {
     var b':bool;
-    LRB.l0 = $[0..q-1];
-    LRB.l  = 0;
+    HybOrcl.l0 = $[0..q-1];
+    HybOrcl.l  = 0;
     b' = A.main();
     return b';
   }
@@ -198,19 +118,16 @@ module B(A:Adv, O:Orcl, LR:LR) = {
 
 section.
 
-  declare module O:Orcl {C, LRB}.
-  declare module A:Adv  {C, O, LRB}.
+  declare module O:Orcl {Count, HybOrcl}.
+  declare module A:Adv  {Count, O, HybOrcl}.
 
-  local module A' (Ob:Orclb, LR:H.Orcl) = {
+  local module A' (Ob : Orclb, LR : H.Orcl) = {
     module O = {
-      proc leaks(il:inleaks) : outleaks = {
-        var r : outleaks;
-        r = Ob.leaks(il);
-        return r;
-      }
+      proc leaks = Ob.leaks
+
       proc orcl(m:input) : output = {
-        var r:output;
-        r = Ob.orcl1((m,m));
+        var r : output;
+        r = Ob.orclL((m,m));
         return r;
       }
     }
@@ -222,8 +139,8 @@ section.
       }
     }
     module A = A(O,LR')
-    proc main():bool = {
-      var b':bool;
+    proc main() : bool = {
+      var b' : bool;
       b' = A.main();
       return b';
     }
@@ -235,98 +152,179 @@ section.
     islossless LR.orcl => 
     islossless O.leaks => islossless O.orcl =>
     islossless A(O, LR).main.
-  axiom q_pos : 0 < q.     
+  axiom q_pos : 0 < q.
          
   lemma IND1_INDn &m (p:glob A -> glob O -> int -> bool):
-     Pr[INDL(O,B(A)).main() @ &m : res /\ p (glob A) (glob O) LRB.l /\
-                                    LRB.l <= q /\ C.c <= 1] - 
-       Pr[INDR(O,B(A)).main() @ &m : res /\ p (glob A) (glob O) LRB.l /\
-                                    LRB.l <= q /\ C.c <= 1]  =
+     Pr[INDL(O,HybGame2(A)).main() @ &m : res /\ p (glob A) (glob O) HybOrcl.l /\
+                                          HybOrcl.l <= q /\ Count.c <= 1] - 
+       Pr[INDR(O,HybGame2(A)).main() @ &m : res /\ p (glob A) (glob O) HybOrcl.l /\
+                                            HybOrcl.l <= q /\ Count.c <= 1]  =
      1%r/q%r * (
-       Pr[INDL(O,A).main() @ &m : res /\ p (glob A) (glob O) C.c /\
-                                  C.c <= q] - 
-         Pr[INDR(O,A).main() @ &m :  res /\ p (glob A) (glob O) C.c /\
-                                  C.c <= q]).
-  proof -strict.
+       Pr[INDL(O,A).main() @ &m : res /\ p (glob A) (glob O) Count.c /\
+                                  Count.c <= q] - 
+         Pr[INDR(O,A).main() @ &m :  res /\ p (glob A) (glob O) Count.c /\
+                                     Count.c <= q]).
+  proof.
     cut := Hybrid (Orcl2(O)) A' _ _ _ _ &m (fun ga go c b, b /\ p ga go c).
-      by proc;call losslessL.
+      by apply losslessL.
       by proc;call losslessO.
       by proc;call losslessO.
       intros Ob LR Hlr Hl Ho1 Ho2;proc.
-      by call (losslessA (<:A'(Ob,LR).O) (<:A'(Ob,LR).LR') _ _ _) => //;proc;
-        [call Hlr | call Hl | call Ho1].
+      call (losslessA (<:A'(Ob,LR).O) (<:A'(Ob,LR).LR') _ _ _) => //;proc.
+        by call Hlr. by call Ho1.
     zeta beta => H.
-    cut -> : Pr[INDL(O, B(A)).main() @ &m :
-                 res /\ p (glob A) (glob O) LRB.l /\ LRB.l <= q /\ C.c <= 1] =
-             Pr[Ln(Orcl2(O), H.B(A')).main() @ &m :
-                 ((res /\ p (glob A) (glob O) LRB.l) /\ LRB.l <= q) /\ C.c <= 1].
+    cut -> : Pr[INDL(O, HybGame2(A)).main() @ &m :
+                 res /\ p (glob A) (glob O) HybOrcl.l /\ HybOrcl.l <= q /\ Count.c <= 1] =
+             Pr[Ln(Orcl2(O), H.HybGame(A')).main() @ &m :
+                 ((res /\ p (glob A) (glob O) HybOrcl.l) /\ HybOrcl.l <= q) /\ Count.c <= 1].
       byequiv (_: ={glob A,glob O} ==>
-                     ={res,glob A,glob O,glob LRB, C.c}) => //;proc.
-      call (_: ={glob A,glob O, C.c} ==> ={glob A,glob O,glob LRB,C.c,res}).
-        proc;inline H.B(A', Orcl2(O), Orclc(L(Orcl2(O)))).A.main;wp.
-        call (_: ={glob O, C.c, glob LRB}).
-          proc *. inline A'(Orcl2(O), LRB(Orcl2(O), Orclc(L(Orcl2(O))))).O.leaks Orcl2(O).leaks;wp.
+                     ={res,glob A,glob O,glob HybOrcl, Count.c}) => //;proc.
+      call (_: ={glob A,glob O, Count.c} ==> ={glob A,glob O,glob HybOrcl,Count.c,res}).
+        proc;inline H.HybGame(A', Orcl2(O), OrclCount(L(Orcl2(O)))).A.main;wp.
+        call (_: ={glob O, Count.c, glob HybOrcl}).
+          proc *. wp.
           by call (_:true);wp.
-          proc *. inline A'(Orcl2(O), LRB(Orcl2(O), Orclc(L(Orcl2(O))))).O.orcl Orcl2(O).orcl1;wp.
+          proc *. inline A'(Orcl2(O), HybOrcl(Orcl2(O), OrclCount(L(Orcl2(O))))).O.orcl Orcl2(O).orclL;wp.
           by call (_:true);wp.
-          proc. inline LRB(Orcl2(O), Orclc(L(Orcl2(O)))).orcl Orcl2(O).orcl1 Orcl2(O).orcl2;wp.
+          proc. inline HybOrcl(Orcl2(O), OrclCount(L(Orcl2(O)))).orcl Orcl2(O).orclL Orcl2(O).orclR;wp.
           sp;if => //;first by wp;call (_:true);wp.
           if => //;last by wp;call (_:true);wp.
-          inline OrclL(O).orcl Orclc(L(Orcl2(O))).orcl L(Orcl2(O)).orcl Orcl2(O).orcl1 C.incr.
+          inline OrclL(O).orcl OrclCount(L(Orcl2(O))).orcl L(Orcl2(O)).orcl Orcl2(O).orclL Count.incr.
           by wp;call (_: true);wp.
         by wp;rnd.
-      by call (_:true ==> ={C.c});first by proc;wp.
-    cut -> : Pr[INDR(O, B(A)).main() @ &m :
-                 res /\ p (glob A) (glob O) LRB.l /\ LRB.l <= q /\ C.c <= 1] =
-             Pr[Rn(Orcl2(O), H.B(A')).main() @ &m :
-                 ((res /\ p (glob A) (glob O) LRB.l) /\ LRB.l <= q) /\ C.c <= 1].
+      by call (_:true ==> ={Count.c});first by proc;wp.
+    cut -> : Pr[INDR(O, HybGame2(A)).main() @ &m :
+                 res /\ p (glob A) (glob O) HybOrcl.l /\ HybOrcl.l <= q /\ Count.c <= 1] =
+             Pr[Rn(Orcl2(O), H.HybGame(A')).main() @ &m :
+                 ((res /\ p (glob A) (glob O) HybOrcl.l) /\ HybOrcl.l <= q) /\ Count.c <= 1].
       byequiv (_: ={glob A,glob O} ==>
-                     ={res,glob A,glob O,glob LRB, C.c}) => //;proc.
-      call (_: ={glob A,glob O, C.c} ==> ={glob A,glob O,glob LRB,C.c,res}).
-        proc;inline H.B(A', Orcl2(O), Orclc(R(Orcl2(O)))).A.main;wp.
-        call (_: ={glob O, C.c, glob LRB}).
-          proc *. inline A'(Orcl2(O), LRB(Orcl2(O), Orclc(R(Orcl2(O))))).O.leaks Orcl2(O).leaks;wp.
+                     ={res,glob A,glob O,glob HybOrcl, Count.c}) => //;proc.
+      call (_: ={glob A,glob O, Count.c} ==> ={glob A,glob O,glob HybOrcl,Count.c,res}).
+        proc;inline H.HybGame(A', Orcl2(O), OrclCount(R(Orcl2(O)))).A.main;wp.
+        call (_: ={glob O, Count.c, glob HybOrcl}).
+          proc *. wp.
           by call (_:true);wp.
-          proc *. inline A'(Orcl2(O), LRB(Orcl2(O), Orclc(R(Orcl2(O))))).O.orcl Orcl2(O).orcl1;wp.
+          proc *. inline A'(Orcl2(O), HybOrcl(Orcl2(O), OrclCount(R(Orcl2(O))))).O.orcl Orcl2(O).orclL;wp.
           by call (_:true);wp.
-          proc. inline LRB(Orcl2(O), Orclc(R(Orcl2(O)))).orcl Orcl2(O).orcl1 Orcl2(O).orcl2;wp.
+          proc. inline HybOrcl(Orcl2(O), OrclCount(R(Orcl2(O)))).orcl Orcl2(O).orclL Orcl2(O).orclR;wp.
           sp;if => //;first by wp;call (_:true);wp.
           if => //;last by wp;call (_:true);wp.
-          inline OrclR(O).orcl Orclc(R(Orcl2(O))).orcl R(Orcl2(O)).orcl Orcl2(O).orcl2 C.incr.
+          inline OrclR(O).orcl OrclCount(R(Orcl2(O))).orcl R(Orcl2(O)).orcl Orcl2(O).orclR Count.incr.
           by wp;call (_: true);wp.
         by wp;rnd.
-      by call (_:true ==> ={C.c});first by proc;wp.
+      by call (_:true ==> ={Count.c});first by proc;wp.
    (* BUG : rewrite H.  *)
-   cut -> : Pr[INDL(O, A).main() @ &m : res /\ p (glob A) (glob O) C.c /\ C.c <= q] =
-            Pr[Ln(Orcl2(O), A').main() @ &m : (res /\ p (glob A) (glob O) C.c) /\ C.c <= q].
+   cut -> : Pr[INDL(O, A).main() @ &m : res /\ p (glob A) (glob O) Count.c /\ Count.c <= q] =
+            Pr[Ln(Orcl2(O), A').main() @ &m : (res /\ p (glob A) (glob O) Count.c) /\ Count.c <= q].
      byequiv (_: ={glob A,glob O} ==>
-                    ={res,glob A,glob O, C.c}) => //;proc.
-      call (_: ={glob A,glob O, C.c} ==> ={glob A,glob O,C.c,res}).
-        proc *. inline A'(Orcl2(O), Orclc(L(Orcl2(O)))).main;sim.
-        call (_: ={glob O, C.c}) => //.
-          proc *. inline A'(Orcl2(O), Orclc(L(Orcl2(O)))).O.leaks Orcl2(O).leaks;wp.
+                    ={res,glob A,glob O, Count.c}) => //;proc.
+      call (_: ={glob A,glob O, Count.c} ==> ={glob A,glob O,Count.c,res}).
+        proc *. inline A'(Orcl2(O), OrclCount(L(Orcl2(O)))).main;sim.
+        call (_: ={glob O, Count.c}) => //.
+          proc *. wp.
           by call (_:true);wp.
-          proc *. inline A'(Orcl2(O), Orclc(L(Orcl2(O)))).O.orcl Orcl2(O).orcl1;wp.
+          proc *. inline A'(Orcl2(O), OrclCount(L(Orcl2(O)))).O.orcl Orcl2(O).orclL;wp.
           by call (_:true);wp.
-          proc;inline Orclc(L(Orcl2(O))).orcl L(Orcl2(O)).orcl Orcl2(O).orcl1 C.incr.
+          proc;inline OrclCount(L(Orcl2(O))).orcl L(Orcl2(O)).orcl Orcl2(O).orclL Count.incr.
         by wp;call(_:true);wp.
-      by call (_:true ==> ={C.c});first by proc;wp.
-   cut -> : Pr[INDR(O, A).main() @ &m : res /\ p (glob A) (glob O) C.c /\ C.c <= q] =
-            Pr[Rn(Orcl2(O), A').main() @ &m : (res /\ p (glob A) (glob O) C.c) /\ C.c <= q].
+      by call (_:true ==> ={Count.c});first by proc;wp.
+   cut -> : Pr[INDR(O, A).main() @ &m : res /\ p (glob A) (glob O) Count.c /\ Count.c <= q] =
+            Pr[Rn(Orcl2(O), A').main() @ &m : (res /\ p (glob A) (glob O) Count.c) /\ Count.c <= q].
      byequiv (_: ={glob A,glob O} ==>
-                    ={res,glob A,glob O, C.c}) => //;proc.
-      call (_: ={glob A,glob O, C.c} ==> ={glob A,glob O,C.c,res}).
-        proc *. inline A'(Orcl2(O), Orclc(R(Orcl2(O)))).main;sim.
-        call (_: ={glob O, C.c}) => //.
-          proc *. inline A'(Orcl2(O), Orclc(R(Orcl2(O)))).O.leaks Orcl2(O).leaks;wp.
+                    ={res,glob A,glob O, Count.c}) => //;proc.
+      call (_: ={glob A,glob O, Count.c} ==> ={glob A,glob O,Count.c,res}).
+        proc *. inline A'(Orcl2(O), OrclCount(R(Orcl2(O)))).main;sim.
+        call (_: ={glob O, Count.c}) => //.
+          proc *. wp.
           by call (_:true);wp.
-          proc *. inline A'(Orcl2(O), Orclc(R(Orcl2(O)))).O.orcl Orcl2(O).orcl1;wp.
+          proc *. inline A'(Orcl2(O), OrclCount(R(Orcl2(O)))).O.orcl Orcl2(O).orclL;wp.
           by call (_:true);wp.
-          proc;inline Orclc(R(Orcl2(O))).orcl R(Orcl2(O)).orcl Orcl2(O).orcl2 C.incr.
+          proc;inline OrclCount(R(Orcl2(O))).orcl R(Orcl2(O)).orcl Orcl2(O).orclR Count.incr.
         by wp;call(_:true);wp.
-      by call (_:true ==> ={C.c});first by proc;wp.
+      by call (_:true ==> ={Count.c});first by proc;wp.
     apply H.
   qed.
 
 end section.
 
+(* -------------------------------------------------------------------- *)
+(* We now prove the equivalence between the two usual definitions *)
+(* i.e (INDb - 1/2) = (INDL - INDR)/2 *)
+
+module Orclb (O:Orcl) = {
+
+  var b:bool
+  proc orcl (m0 m1:input) : output = {
+    var r : output;
+    Count.incr();
+    r <@ O.orcl(b?m0:m1);
+    return r;
+  }
+}.
+
+module INDb(O:Orcl,A:Adv) = {
+  module A = A(O,Orclb(O))
+  proc main():bool = {
+    var b' : bool;
+    Count.init();
+    Orclb.b <$ {0,1};
+    b' <@ A.main();
+    return Orclb.b = b';
+  }
+}.
+
+section.
+  declare module O:Orcl {Count, Orclb}.
+  declare module A:Adv  {Count, O, Orclb}.
+
+  local module WA = {
+    module A = A(O,Orclb(O))
+    proc work(x : bool) : bool = {
+      var b' : bool;
+      Count.init();
+      Orclb.b <- x;
+      b' <@ A.main();
+      return b';
+    }
+  }.
+
+  lemma INDb_INDLR &m (p:glob A -> glob O -> int -> bool):
+     Pr[INDb(O,A).main() @ &m : res /\ p (glob A) (glob O) Count.c] -
+       Pr[INDR(O,A).main() @ &m : p (glob A) (glob O) Count.c]/2%r =
+     (Pr[INDL(O,A).main() @ &m : res /\ p (glob A) (glob O) Count.c] -
+      Pr[INDR(O,A).main() @ &m : res /\ p (glob A) (glob O) Count.c])/2%r.
+  proof.
+   cut := Sample_bool WA &m 
+     (fun (g:glob WA), let (b,c,ga,go) = g in p ga go c) => /= H.
+   cut -> : Pr[INDb(O, A).main() @ &m : res /\ p (glob A) (glob O) Count.c] =
+    Pr[MB.M.Rand(WA).main() @ &m : fst res = snd res /\ p (glob A) (glob O) Count.c].
+     byequiv (_: ={glob A,glob O} ==> ={glob A,glob O, Count.c} /\
+                   res{1} = (fst res = snd res){2}) => //;proc.
+     inline Count.init WA.work;simplify fst snd. 
+     by swap{1} 2 -1; sim; proc (={Orclb.b, Count.c}).
+   cut He: equiv [INDR(O, A).main ~ WA.work: x{2}=false /\ 
+                   ={glob A,glob O} ==> ={res,glob A,glob O, Count.c}].
+    proc. 
+    call (_: ={glob O, Count.c} /\ Orclb.b{2} = false).
+      by proc (={Count.c} /\ Orclb.b{2} = false).      
+      by proc (={Count.c} /\ Orclb.b{2} = false). 
+      by proc;inline Count.incr;wp;call(_:true);wp;skip;progress.
+    inline Count.init;by wp.
+   cut -> : Pr[INDR(O, A).main() @ &m : p (glob A) (glob O) Count.c] =
+            Pr[WA.work(false) @ &m : p (glob A) (glob O) Count.c].
+     by byequiv He.
+   cut -> : Pr[INDR(O, A).main() @ &m : res /\ p (glob A) (glob O) Count.c] = 
+            Pr[WA.work(false) @ &m : res /\ p (glob A) (glob O) Count.c].
+     by byequiv He.
+   (cut -> : Pr[INDL(O, A).main() @ &m : res /\ p (glob A) (glob O) Count.c] = 
+            Pr[WA.work(true) @ &m : res /\ p (glob A) (glob O) Count.c]) => //.
+   byequiv 
+      (_: x{2}=true /\ ={glob A,glob O} ==> ={res,glob A,glob O, Count.c}) => //.
+   proc; call (_: ={glob O, Count.c} /\ Orclb.b{2} = true).
+     by proc (={Count.c} /\ Orclb.b{2} = true).      
+     by proc (={Count.c} /\ Orclb.b{2} = true). 
+     by proc;inline Count.incr;wp;call(_:true);wp;skip;progress.
+   inline Count.init;by wp.
+ qed.
+
+end section.
